<?xml version="1.0" encoding="UTF-8"?>
<rdf:RDF xmlns="http://www.cyc.com/2004/06/04/cyc#"
    xmlns:owl="http://www.w3.org/2002/07/owl#"
    xmlns:rdf="http://www.w3.org/1999/02/22-rdf-syntax-ns#" 
    xmlns:rdfs="http://www.w3.org/2000/01/rdf-schema#">
    <owl:Ontology rdf:about="">
        <owl:versionInfo>$Id: DistrES.java,v 0.1 2005/04/25
            fergus Exp $</owl:versionInfo>
        <rdfs:comment>ResearchCyc Ontology  OpenCyc License Information
            The contents of this file constitute portions of The OpenCyc
            Knowledge Base. The OpenCyc Knowledge Base is protected
            under the following license and copyrights. This license and
            copyright information must be included with any copies or
            derivative works.  Copyright Information OpenCyc Knowledge
            Base Copyright 2001-2004 Cycorp, Inc., Austin, TX, USA. All
            rights reserved. OpenCyc Knowledge Server Copyright
            2001-2004 Cycorp, Inc., Austin, TX, USA. All rights
            reserved. Other copyrights may be found in various files.
            The OpenCyc Knowledge Base The OpenCyc Knowledge Base
            consists of code, written in the declarative language CycL,
            that represents or supports the representation of facts and
            rules pertaining to consensus reality. OpenCyc is licensed
            using the GNU Lesser General Public License, whose text can
            also be found on this volume. The OpenCyc CycL code base is
            the &quot;library&quot; referred to in the LGPL license. The
            terms of this license equally apply to renamings and other
            logically equivalent reformulations of the Knowledge Base
            (or portions thereof) in any natural or formal language.
            See http://www.opencyc.org for more information. 
		
		This ontology is used by DistrES. For know
		every device that implements the DistrES ontology will
		implement this ontology. For experimental purposes this
		ontology contains the concepts associated with all the 
		functions provided by each device within the network.
		In reality this ontology woul only contain concepts 
		directly relating to the functions the device provides.
		For example if this ontology was to be used by a speaker
		then the only concepts that it would contain would be 
		concepts relating the funnctions provided by a speaker.</rdfs:comment>
    </owl:Ontology>

    <!-- All subClassOf associations checked -->
    <owl:Class rdf:ID="AccessingCDROMData">
        <rdfs:comment>An #$EmployeeComputerActivityType and a
            specialization of #$DataSending.  This is the collection of
            #$Events in which data is accessed from a CD through a
            #$CD-ROMDriver and sent to some output device.</rdfs:comment>
        <rdf:type rdf:resource="#EmployeeComputerActivityType"/>
        <rdfs:subClassOf rdf:resource="#ComputerActivity"/>
        <rdfs:subClassOf rdf:resource="#DataSending"/>
    </owl:Class>

    <!-- All subClassOf associations checked -->
    <owl:Class rdf:ID="AccessingData-DivX">
        <rdfs:comment>A specialization of #$DataSending. Each instance
            of this collection is an #$Event in which data is accessed
            from a #$DivXFileCopy and sent to some output device.</rdfs:comment>
        <rdf:type rdf:resource="#EmployeeComputerActivityType"/>
        <rdfs:subClassOf rdf:resource="#DataSending"/>
        <rdfs:subClassOf rdf:resource="#ComputerActivity"/>
    </owl:Class>

    <!-- All subClassOf associations checked -->
    <owl:Class rdf:ID="AccessingData-DVD">
        <rdfs:comment>A specialization of #$DataSending. Each instance
            of this collection is an #$Event in which data is accessed
            from a #$DVD-Disk, perhaps also interacting with a
            #$DVDPlayer device, and sent to some output device.</rdfs:comment>
        <rdf:type rdf:resource="#EmployeeComputerActivityType"/>
        <rdfs:subClassOf rdf:resource="#ComputerActivity"/>
        <rdfs:subClassOf rdf:resource="#DataSending"/>
    </owl:Class>

    <!-- All subClassOf associations checked -->
    <owl:Class rdf:ID="AccessingData-MP3">
        <rdfs:comment>A specialization of #$DataSending. Each instance
            of this collection is an #$Event in which data is accessed
            from a #$MP3FileCopy and sent to some output device.</rdfs:comment>
        <rdf:type rdf:resource="#EmployeeComputerActivityType"/>
        <rdfs:subClassOf rdf:resource="#DataSending"/>
        <rdfs:subClassOf rdf:resource="#ComputerActivity"/>
    </owl:Class>

    <!-- All subClassOf associations checked -->
    <owl:Class rdf:ID="AccessingData-VCD">
        <rdfs:comment>A specialization of #$DataSending. Each instance
            of this collection is an #$Event in which data is accessed
            from a #$VCDFileCopy and sent to some output device.</rdfs:comment>
        <rdf:type rdf:resource="#EmployeeComputerActivityType"/>
        <rdfs:subClassOf rdf:resource="#DataSending"/>
        <rdfs:subClassOf rdf:resource="#ComputerActivity"/>
    </owl:Class>

    <!-- All subClassOf associations checked -->
    <owl:Class rdf:ID="AccessingData-Xvid">
        <rdfs:comment>A specialization of #$DataSending. Each instance
            of this collection is an #$Event in which data is accessed
            from a #$MP3FileCopy and sent to some output device.</rdfs:comment>
        <rdf:type rdf:resource="#EmployeeComputerActivityType"/>
        <rdfs:subClassOf rdf:resource="#DataSending"/>
        <rdfs:subClassOf rdf:resource="#ComputerActivity"/>
    </owl:Class>

    <!-- All subClassOf associations checked -->
    <owl:Class rdf:ID="Action">
        <rdfs:comment>The collection of #$Events (q.v.) that are carried
            out by some  doer  (see #$doneBy).  Instances of #$Action
            include any event in which one or more actors effect some
            change in the (tangible or intangible) state of the world,
            typically by an expenditure of effort or energy.  Note that
            it is not required that any tangible object be moved,
            changed, produced, or destroyed for an action to occur; the
            effects of an action might be intangible (such as a change
            in a bank balance or the intimidation of a subordinate).
            Note also that the doer of an action, though typically an
            #$Agent (q.v.), need not be (e.g. a falling rock that dents
            a car&apos;s roof).  Depending upon the context, doers of
            actions might be animate or inanimate, conscious or
            nonconscious.  For actions that are intentional, see
            #$PurposefulAction and #$performedBy.</rdfs:comment>
        <rdf:type rdf:resource="#CDETagTranslationConstant"/>
        <rdfs:subClassOf rdf:resource="http://www.w3.org/2002/07/owl#Thing"/>
        <rdfs:subClassOf rdf:resource="#Event"/>
    </owl:Class>

    <!-- All subClassOf associations checked -->
    <owl:Class rdf:ID="Amplifier">
        <rdfs:comment>A collection of devices; a subset of
            ElectronicComponent. Each instance of Amplifier is a device
            used for   increasing the amplitude of a signal passing
            through it.</rdfs:comment>
        <rdf:type rdf:resource="#ManufacturedGoodsType"/>
        <rdfs:subClassOf rdf:resource="#ManufacturedGoods"/>
        <rdfs:subClassOf rdf:resource="#ElectronicComponent"/>
    </owl:Class>

    <!-- All subClassOf associations checked -->
    <owl:Class rdf:ID="AudioAmplifierComponent">
        <rdfs:comment>Electronic Device which amplifies electrical audio signals.</rdfs:comment>
        <rdf:type rdf:resource="#ManufacturedGoodsType"/>
        <rdfs:subClassOf rdf:resource="#Amplifier"/>
        <rdfs:subClassOf rdf:resource="#ConsumerAudioVideoComponent"/>
    </owl:Class>

    <!-- All subClassOf associations checked -->
    <owl:Class rdf:ID="AudioCommunicating">
        <rdfs:comment>A specialization of #$Communicating.  Each
            instance of #$AudioCommunicating is a transmission of
            sound-borne information between two (or more) agents.
            Specializations of #$AudioCommunicating include
            #$SpokenCommunicating and #$MusicalCommunicating.</rdfs:comment>
        <rdfs:subClassOf rdf:resource="#Communicating"/>
    </owl:Class>

    <!-- All subClassOf associations checked -->
    <owl:Class rdf:ID="AudioCrossover">
        <rdfs:comment>This is the collection of crossovers. A crossover
            is a piece of #$AudioEquipment  designed to process audio
            signals in the frequency ranges where different  drivers
            have frequency overlaps.</rdfs:comment>
        <rdfs:subClassOf rdf:resource="#Amplifier"/>
    </owl:Class>

    <!-- All subClassOf associations checked -->
    <owl:Class rdf:ID="AudioEquipment">
        <rdfs:comment>A collection of electronic devices.  An instance
            of #$AudioEquipment is a device that may be used in audio
            recording, playback, amplification, and/or reception.  This
            collection doesn&apos;t include musical instruments.  It
            does include both self-contained systems, e.g. boom boxes,
            and individual stereo components, such as microphones,
            amplifiers, etc.</rdfs:comment>
        <rdfs:subClassOf rdf:resource="#ElectronicDevice"/>
    </owl:Class>

    <!-- All subClassOf associations checked -->
    <owl:Class rdf:ID="AudioRecordedObject">
        <rdfs:comment>A collection of information bearing objects
            (IBOs).  Each element of #$AudioRecordedObject is a tangible
            object (such as an audiocassette tape) that contains audio
            information.  For mass-produced audio, see #$RecordedSoundProduct.</rdfs:comment>
    </owl:Class>

    <!-- All subClassOf associations checked -->
    <owl:Class rdf:ID="AudioSpeaker">
        <rdfs:comment>The electrical component used to convey sound</rdfs:comment>
        <rdf:type rdf:resource="#ManufacturedGoodsType"/>
        <rdfs:subClassOf rdf:resource="#ManufacturedGoods"/>
        <rdfs:subClassOf rdf:resource="#ElectricalComponent"/>
    </owl:Class>

    <!-- All subClassOf associations checked -->
    <owl:Class rdf:ID="AudioSystem">
        <rdfs:comment>The collection of all audio systems, characterized
            by having an audio amplifier, some kind of speaker (which
            may be headphones), and some sound producing component such
            as a radio receiver or tape deck mechanism.</rdfs:comment>
        <rdfs:subClassOf rdf:resource="#AudioEquipment"/>
        <rdfs:subClassOf rdf:resource="#System"/>
    </owl:Class>

    <!-- All subClassOf associations checked -->
    <owl:Class rdf:ID="AudioSystemComponent">
        <rdfs:comment>The collection of audio components intended for
            use in an #$AudioSystem.  Each instance of #$AudioSystem has
            several instances of #$AudioSystemComponent as
            #$physicalParts.  No instance of #$AudioSystemComponent is
            itself an instance of #$AudioSystem.</rdfs:comment>
        <rdfs:subClassOf rdf:resource="#AudioEquipment"/>
    </owl:Class>

    <!-- All subClassOf associations checked -->
    <owl:Class rdf:ID="AudioVisualReceiver">
        <rdfs:comment>This is the collection of single-unit  receivers
            for #$HomeTheaterSystems.</rdfs:comment>
        <rdf:type rdf:resource="#ManufacturedGoodsType"/>
        <rdfs:subClassOf rdf:resource="#Receiver-AudioComponent"/>
        <rdfs:subClassOf rdf:resource="#VideoReceiverComponent"/>
        <rdfs:subClassOf rdf:resource="#ElectronicDevice"/>
    </owl:Class>

    <!-- All subClassOf associations checked -->
    <owl:Class rdf:ID="BidirectionalDataStream">
        <rdfs:comment>This generic data type encapsluates the concept of
            bidirectional streams (allowing both input and output) in
            programming languages.</rdfs:comment>
        <rdf:type rdf:resource="#ComputerDataType"/>
        <rdfs:subClassOf rdf:resource="#DataStream"/>
    </owl:Class>

    <!-- All subClassOf associations checked -->
    <owl:Class rdf:ID="CDPlayer-AudioComponent">
        <rdfs:comment>The device used to play compact discs</rdfs:comment>
        <rdf:type rdf:resource="#ManufacturedGoodsType"/>
        <rdfs:subClassOf rdf:resource="#CompactDiscPlayer"/>
        <rdfs:subClassOf rdf:resource="#ConsumerAudioVideoComponent"/>
    </owl:Class>

    <!-- All subClassOf associations checked -->
    <owl:Class rdf:ID="CellularTelephone">
        <rdfs:comment>Cellular mobile telephone unit usually used in automobiles</rdfs:comment>
        <rdf:type rdf:resource="#ContactLocationType"/>
        <rdf:type rdf:resource="#ManufacturedGoodsType"/>
        <rdfs:subClassOf rdf:resource="#ManufacturedGoods"/>
        <rdfs:subClassOf rdf:resource="#WirelessCommunicationDevice"/>
        <rdfs:subClassOf rdf:resource="#PersonalDevice"/>
    </owl:Class>

    <!-- All subClassOf associations checked -->
    <owl:Class rdf:ID="Communicating">
        <rdfs:comment>A specialization of #$PurposefulAction and
            characterized by one or more #$InformationTransferEvent
            sub-events.  Each instance of #$Communicating is an event in
            which the transfer of information between or among agents is
            a focal action; communicating is the main purpose and/or
            goal in the event.  That may be contrasted with events which
            involve communication but wherein the focus is different,
            e.g., playing cards (wherein the progressive actions -- and
            winning -- of the game are focal).  Since #$Communicating is
            a specialization of #$PurposefulAction, each #$Communicating
            event must be intentional on the part of the
            #$communicatorOfInfo; it may or may not be intentional on
            the part of the agent playing the #$infoCommunicatedTo role.
            Hence, a speaker on a soapbox haranguing an indifferent
            crowd is performing an instance of #$Communicating.  In
            contrast, Juliet soliloquizing on her balcony, unaware that
            Romeo is listening to her, is not #$Communicating; rather
            Romeo (and Juliet, unaware) are engaged in an
            #$Eavesdropping. Communicating may be either a one-way or a
            two-way transfer of information (cf.
            #$CommunicationAct-Single, #$MultiDirectionalCommunication).
            Every event belonging to #$Communicating contains at least
            one transfer of information between at least two agents who
            participate in the event.  (Note that the latter requirement
            excludes reading and writing from #$Communicating, when
            those events are just the private accessing or generating of
            information.)  Communicating may be specialized in various
            ways, such as, by the method or medium used (e.g.,
            #$AudioCommunicating, #$NonVerbalCommunicating,
            #$FaceToFacePresenceCommunicating); by the type of
            information involved (e.g., #$MakingAnAgreement); by the
            purpose of the communication (e.g., #$Teaching,
            #$Negotiating); by the agents involved (e.g.,
            #$IntraOrganizationCommunication, #$StageProduction).
            Examples of #$Communicating include a symphony performance,
            an email message, a telephone call, a speech, a handshake,
            issuing a traffic ticket -- all of which normally, and
            focally, involve communication between two or more agents.</rdfs:comment>
    </owl:Class> 

    <!-- All subClassOf associations checked -->
    <owl:Class rdf:ID="CommunicationDevice">
        <rdfs:comment>The subcollection of #$PhysicalDevice that
            contains all instances that are intended to be the
            #$deviceUsed in a #$Communicating (one way or
            bidirectional). Examples include #$RadioReceiver,
            #$Telephone, etc.</rdfs:comment>
        <rdfs:subClassOf rdf:resource="#PhysicalDevice"/>
    </owl:Class>

    <!-- All subClassOf associations checked -->
    <owl:Class rdf:ID="CompactDisc-Audio">
        <rdfs:comment>A specialization of #$CompactDisc-Generic.  Each
            instance of this collection is designed to be used for
            storing audio in the CD format, which is most commonly used
            for music.</rdfs:comment>
        <rdf:type rdf:resource="#ManufacturedGoodsType"/>
        <rdfs:subClassOf rdf:resource="#CompactDisc-Generic"/>
    </owl:Class>

    <!-- All subClassOf associations checked -->
    <owl:Class rdf:ID="CompactDisc-Generic">
        <rdfs:comment>The collection of generic CompactDiscs often (but
            not  necessarily) used for digital information storage,
            whether audio,  video or other.  Subcollections include
            #$CompactDisc-Audio,  #$CD-ROM, #$CD-R, #$CD-RW, etc..</rdfs:comment>
        <rdf:type rdf:resource="#ManufacturedGoodsType"/>
        <rdfs:subClassOf rdf:resource="#DiscStorageMedium"/>
    </owl:Class>

    <!-- All subClassOf associations checked -->
    <owl:Class rdf:ID="CompactDiscPlayer">
        <rdfs:comment></rdfs:comment>
        <rdf:type rdf:resource="#ManufacturedGoodsType"/>
        <rdfs:subClassOf rdf:resource="#ManufacturedGoods"/>
        <rdfs:subClassOf rdf:resource="#AudioEquipment"/>
        <rdfs:subClassOf rdf:resource="#MediaPlayingDevice"/>
    </owl:Class>

    <!-- All subClassOf associations checked -->
    <owl:Class rdf:ID="CompactStereoSystem">
        <rdfs:comment>A subcollection of #$HomeAudioSystem. Instances of
            #$CompactStereoSystem are on the physically small and
            inexpensive end.</rdfs:comment>
        <rdf:type rdf:resource="#ManufacturedGoodsType"/>
        <rdfs:subClassOf rdf:resource="#ManufacturedGoods"/>
        <rdfs:subClassOf rdf:resource="#HomeAudioSystem"/>
    </owl:Class>

    <!-- All subClassOf associations checked -->
    <owl:Class rdf:ID="ComputerActivity">
        <rdfs:comment>A collection of events, and a specialization of
            both #$Action and #$PhysicalEvent. In each instance of
            #$ComputerActivity, at least one instance of #$Computer is
            somehow involved. An instance of #$Person may or may not be
            involved. (Instances of #$ComputerActivity where no #$Person
            is involved fall under the more specialized collection
            #$ComputerProcessRunning.) A wide variety of activities
            falls into this collection - from sending an email (see the
            more specialized collection #$EMailSending), to scanning a
            set of ports (see #$PortScan), to a computer crash (see
            #$ComputerCrashing). A situation where someone took to a
            computer with an axe would also fulfil the requirements for
            being an instance of #$ComputerActivity, though (hopefully)
            in an unusual and &apos;degenerate&apos; sense.</rdfs:comment>
        <rdfs:subClassOf rdf:resource="#PhysicalEvent"/>
        <rdfs:subClassOf rdf:resource="#Action"/>
    </owl:Class>

    <!-- All subClassOf associations checked -->
    <owl:Class rdf:ID="ComputerDisk">
        <rdfs:comment>A spec of #$InformationStorageMedia, this is the
            collection of all disks used for storage of information.
            This includes floppy disks as well as hard disks.</rdfs:comment>
        <rdf:type rdf:resource="#ManufacturedGoodsType"/>
        <rdfs:subClassOf rdf:resource="#DiscStorageMedium"/>
        <rdfs:subClassOf rdf:resource="#ComputerInformationStorageMedia"/>
        <rdfs:subClassOf rdf:resource="#ComputerHardwareItem"/>
    </owl:Class>

    <owl:Class rdf:ID="ComputerDisplay">
        <rdfs:comment>A specialization of #$ComputerOutputDevice. Each
            instance of this collection is a device with which computer
            output is displayed visually. An important specialization is
            #$ComputerMonitor-VideoKind, but see also #$DataProjector.</rdfs:comment>
        <rdf:type rdf:resource="#ManufacturedGoodsType"/>
        <rdfs:subClassOf rdf:resource="#ElectronicDisplayDevice"/>
        <rdfs:subClassOf rdf:resource="#ComputerOutputDevice"/>
    </owl:Class>

    <!-- All subClassOf associations checked -->
    <owl:Class rdf:ID="ComputerHardwareComponent">
        <rdfs:comment></rdfs:comment>
        <rdf:type rdf:resource="#ManufacturedGoodsType"/>
        <rdfs:subClassOf rdf:resource="#ComputerHardwareItem"/>
    </owl:Class>

    <!-- All subClassOf associations checked -->
    <owl:Class rdf:ID="ComputerHardwareItem">
        <rdfs:comment>A specialization of #$ElectronicDevice and
            #$ComputerProduct. Each instance of this collection is
            either an entire #$Computer, or a device used with or in
            computers to accomplish some computing-related task (for
            instance, computer terminals, printers, keyboards, etc.).</rdfs:comment>
        <rdfs:subClassOf rdf:resource="#ManufacturedGoods"/>
        <rdfs:subClassOf rdf:resource="#ElectronicDevice"/>
    </owl:Class>

    <!-- All subClassOf associations checked -->
    <owl:Class rdf:ID="ComputerInformationStorageMedia">
        <rdfs:comment>#$ComputerInformationStorageMedia is the subset of
            #$InformationStorageMedia whose instances are all and only
            those entities on which instances of #$ComputerFileCopy may
            be stored.</rdfs:comment>
        <rdf:type rdf:resource="#ObjectType"/>
        <rdfs:subClassOf rdf:resource="#InformationStorageMedia"/>
    </owl:Class>

    <!-- All subClassOf associations checked -->
    <owl:Class rdf:ID="ComputerInterfaceDevice">
        <rdfs:comment>A specialization of #$ElectronicDevice. Each
            instance of this collection is a device that allows a user
            to communicate with a #$Computer.  One sigificant
            specialization of #$ComputerInterfaceDevices is
            #$ComputerInputDevice -- with its subsets
            #$ComputerKeyboard, #$Scanner-Optical, #$ComputerMouse, etc.
            Another is #$ComputerOutputDevice -- with its subsets
            #$MonitorPort, #$ComputerMonitor-Color, etc.</rdfs:comment>
        <rdf:type rdf:resource="#ManufacturedGoodsType"/>
        <rdfs:subClassOf rdf:resource="#ComputerHardwareComponent"/>
    </owl:Class>

    <!-- All subClassOf associations checked -->
    <owl:Class rdf:ID="ComputerMonitor-BlackAndWhite">
        <rdfs:comment></rdfs:comment>
        <rdf:type rdf:resource="#ManufacturedGoodsType"/>
        <rdfs:subClassOf rdf:resource="#ComputerMonitor-VideoKind"/>
    </owl:Class>

    <!-- All subClassOf associations checked -->
    <owl:Class rdf:ID="ComputerMonitor-Color">
        <rdfs:comment></rdfs:comment>
        <rdf:type rdf:resource="#ManufacturedGoodsType"/>
        <rdfs:subClassOf rdf:resource="#ComputerMonitor-VideoKind"/>
    </owl:Class>

    <!-- All subClassOf associations checked -->
    <owl:Class rdf:ID="ComputerMonitor-VideoKind">
        <rdfs:comment>Like the screen you are staring at.  Don&apos;t
            confuse with ComputerDisplay.</rdfs:comment>
        <rdf:type rdf:resource="#ManufacturedGoodsType"/>
        <rdfs:subClassOf rdf:resource="#ComputerDisplay"/>
    </owl:Class>

    <!-- All subClassOf associations checked -->
    <owl:Class rdf:ID="ComputerOutputDevice">
        <rdfs:comment>A specialization of #$ComputerInterfaceDevice.
            Each instance of this collection is an #$ElectronicDevice
            which delivers information from a computer to its user.</rdfs:comment>
        <rdf:type rdf:resource="#ManufacturedGoodsType"/>
        <rdfs:subClassOf rdf:resource="#ComputerInterfaceDevice"/>
    </owl:Class>

    <!-- All subClassOf associations checked -->
    <owl:Class rdf:ID="ConsumerAudioVideoComponent">
        <rdfs:comment>The collection of all
            #$ElectronicHouseholdAppliances that are sold to be
            components in a home audio or audio-video system. Instances
            of #$ConsumerAudioVideoComponent are generally black in
            color and of a fairly uniform size, so they are visually
            inconspicuous and can be installed in standard cabinets.
            They are generally connected to one another using patch cords.</rdfs:comment>
        <rdfs:subClassOf rdf:resource="#ElectronicHouseholdAppliance"/>
    </owl:Class>

    <!-- All subClassOf associations checked -->
    <owl:Class rdf:ID="DataSending">
        <rdfs:comment>This is a collection of one-way information
            transfer events in which information  is sent from some
            #$informationOrigin to some #$informationDestination.</rdfs:comment>
        <rdfs:subClassOf rdf:resource="#InformationTransferPhysicalEvent"/>
    </owl:Class>

    <!-- All subClassOf associations checked -->
    <owl:Class rdf:ID="DataSignaling">
        <rdfs:comment>This is the collection of all events in which
            information is passed from a source to a target by
            non-obvious means.  This is usually done to avoid some form
            of security monitoring.</rdfs:comment>
        <rdfs:subClassOf rdf:resource="#DataSending"/>
    </owl:Class>

    <!-- All subClassOf associations checked -->
    <owl:Class rdf:ID="DataStream">
        <rdfs:comment>This generic data type encapsluates the concept of
            streams in programming languages. This includes all streams,
            including Input and Output streams, as well as Byte and
            Character streams.</rdfs:comment>
        <rdf:type rdf:resource="#ComputerDataType"/>
        <rdfs:subClassOf rdf:resource="#ProgramObject"/>
    </owl:Class>

    <!-- All subClassOf associations checked -->
    <owl:Class rdf:ID="DecoderProgram">
        <rdfs:comment>The collection of all #$ComputerProgram-CWs whose
            purpose         is to perform an #$IBTRecoding with a
            #$ComputerFileCopy as its         #$informationOrigin and an
            #$InformationBearingThing containing         the same
            information as its #$ibtGenerated. See #$EncoderProgram
            for programs going the other direction.</rdfs:comment>
        <rdf:type rdf:resource="#ComputerProgramTypeByFunction"/>
        <rdfs:subClassOf rdf:resource="#UtilityProgram"/>
    </owl:Class>

    <!-- All subClassOf associations checked -->
    <owl:Class rdf:ID="Decoding">
        <rdfs:comment>The collection of events where some data in an
            #$InformationBearingThing are transformed from a
            complex/compressed format to a more usable or natural format.</rdfs:comment>
    </owl:Class>

    <!-- All subClassOf associations checked -->
    <owl:Class rdf:ID="Device-SingleUser">
        <rdfs:comment>#$Device-SingleUser is a specialization of
            #$PhysicalDevice.  Each instance of #$Device-SingleUser is a
            device that typically has exactly one (i.e., one and only
            one)  user  who is the only individual who derives the value
            of its single function at a single time.  A screwdriver (an
            instance of  #$Screwdriver) is a #$Device-SingleUser, but a
            grand piano (an instance of #$GrandPiano) is not.  A
            borderline non-example is a multiple-passenger car ---
            although only one person operates it, several can  use  it
            at once, i.e. derive the value of its primary function
            (transportation).  So a multiple-passenger car is not a
            #$Device-SingleUser. A borderline example is a telephone --
            although it requires two or more users (each on telephones)
            for meaningful use, each phone generally has just one user
            at a time.  So a telephone is a #$Device-SingleUser, but a
            telephone-circuit is not.</rdfs:comment>
        <rdfs:subClassOf rdf:resource="#PhysicalDevice"/>
    </owl:Class>  

    <!-- All subClassOf associations checked -->
    <owl:Class rdf:ID="Disc">
        <rdfs:comment>A specialization of #$Cylinder. Each instance of
            #$Disc3DShape is a cylinder with a height much less than the
            radius of its base.</rdfs:comment>
        <rdf:type rdf:resource="#ThreeDimensionalShapeType"/>
    </owl:Class>

    <!-- All subClassOf associations checked -->
    <owl:Class rdf:ID="DiscStorageMedium">
        <rdfs:comment>A spec of #$InformationStorageMedia, this is the
            collection of all disks used for storage of information.
            This includes floppy disks as well as hard disks.</rdfs:comment>
        <rdf:type rdf:resource="#ManufacturedGoodsType"/>
        <rdfs:subClassOf rdf:resource="#ManufacturedGoods"/>
        <rdfs:subClassOf rdf:resource="#Disc"/>
        <rdfs:subClassOf rdf:resource="#InformationStorageMedia"/>
        <rdfs:subClassOf rdf:resource="#PhysicalDevice"/>
    </owl:Class>

    <!-- All subClassOf associations checked -->
    <owl:Class rdf:ID="DVD-Disk">
        <rdfs:comment>A collection of #$Disks. Each #$DVD-Disk is a
            round, shiny disk similar in shape and appearance to a
            #$CompactDisc-Generic, but with a greater storage capacity
            (several gigabytes, depending on whether it is single- or
            double-sided and how many layers of information are encoded
            on each side). #$DVD-Disks are currently (1998) used for
            distribution and playback of #$Movie-CWs and multimedia
            software too large for #$CD-ROMs, and for backup of computer #$HardDiskDrives.</rdfs:comment>
        <rdf:type rdf:resource="#ComputerDiskType"/>
        <rdfs:subClassOf rdf:resource="#ComputerDisk"/>
        <rdfs:subClassOf rdf:resource="#SinglePurposeDevice"/>
    </owl:Class>

    <!-- All subClassOf associations checked -->
    <owl:Class rdf:ID="DVDPlayer">
        <rdfs:comment>A #$DVDPlayer is a type of home audio-visual
            equipment,  for playing #$DVD-Disks. See also #$DVDPlayer-Software.</rdfs:comment>
        <rdf:type rdf:resource="#ManufacturedGoodsType"/>
        <rdfs:subClassOf rdf:resource="#ManufacturedGoods"/>
        <rdfs:subClassOf rdf:resource="#ConsumerAudioVideoComponent"/>
        <rdfs:subClassOf rdf:resource="#MediaPlayingDevice"/>
    </owl:Class>

    <!-- All subClassOf associations checked -->
    <owl:Class rdf:ID="ElectricalComponent">
        <rdfs:comment>A specialization of both #$ElectricalDevice and
            #$PhysicalPartOfObject.  Each instance of
            #$ElectricalComponent is an #$ElectricalDevice which is
            normally considered to be a part of some larger, more
            clearly distinguished #$PhysicalDevice (for example, clearly
            distinguished in the sense that it is sold or moved as a
            unit).  Each instance of  #$ElectricalComponent must be
            connected with other parts in order to perform its #$primaryFunction.</rdfs:comment>
        <rdfs:subClassOf rdf:resource="#ElectricalDevice"/>
    </owl:Class>

    <!-- All subClassOf associations checked -->
    <owl:Class rdf:ID="ElectricalDevice">
        <rdfs:comment>A specialization of #$PoweredDevice.  Each
            instance of #$ElectricalDevice is a device that requires an
            input of electrical current (as its #$energySource) in order
            to perform its intended function(s).  Instances of
            #$ElectricalDevice include both complex devices (for
            example, instances of the collections #$StereoSystem or
            #$Computer) and simpler ones (for example, instances of the
            collection #$ElectricalComponent).</rdfs:comment>
        <rdfs:subClassOf rdf:resource="#PoweredDevice"/>
    </owl:Class>

    <!-- All subClassOf associations checked -->
    <owl:Class rdf:ID="ElectricalHouseholdAppliance">
        <rdfs:comment>Electric-powered Household Appliances</rdfs:comment>
        <rdfs:subClassOf rdf:resource="#ElectricalDevice"/>
        <rdfs:subClassOf rdf:resource="#HouseholdAppliance"/>
    </owl:Class>

    <!-- All subClassOf associations checked -->
    <owl:Class rdf:ID="ElectronicComponent">
        <rdfs:comment>A collection of devices; a subset of
            #$ElectronicDevice.  An #$ElectronicComponent is a device
            which is normally considered a part to another device (which
            in turn is a more meaningful entity, at least in this
            context.  `More meaningful&apos; might mean that the larger
            device is sold, moved, named,... as a unit.)   An electronic
            component needs to be connected with other parts in order to
            perform its #$primaryFunction.</rdfs:comment>
        <rdfs:subClassOf rdf:resource="#ElectricalComponent"/>
        <rdfs:subClassOf rdf:resource="#ElectronicDevice"/>
    </owl:Class>

    <!-- All subClassOf associations checked -->
    <owl:Class rdf:ID="ElectronicDevice">
        <rdfs:comment>#$ElectronicDevice is a specialization of
            #$ElectricalDevice.  Each instance of #$ElectronicDevice is
            a device that uses electronic circuitry; more specifically,
            a device in which electricity passes through a vacuum or
            semiconductor.  Notable specializations of
            #$ElectronicDevice include #$Telephone, #$VideoCamera, and #$Computer.</rdfs:comment>
        <rdfs:subClassOf rdf:resource="#ElectricalDevice"/>
    </owl:Class>

    <!-- All subClassOf associations checked -->
    <owl:Class rdf:ID="ElectronicDisplayDevice">
        <rdfs:comment>Electronic devices used to display images.  E.g.
            CRTs and LCDs.</rdfs:comment>
        <rdf:type rdf:resource="#ManufacturedGoodsType"/>
        <rdfs:subClassOf rdf:resource="#ManufacturedGoods"/>
        <rdfs:subClassOf rdf:resource="#ElectronicComponent"/>
    </owl:Class>

    <!-- All subClassOf associations checked -->
    <owl:Class rdf:ID="ElectronicHouseholdAppliance">
        <rdfs:comment>A collection of electronic devices which are also
            household appliances.  An instance of
            #$ElectronicHouseholdAppliance is a #$HouseholdAppliance
            which is electrically powered and controlled.  Common
            instances of #$ElectronicHouseholdAppliance belong to the
            subsets #$HomeVideoGameMachine, #$TelevisionSet,
            #$AnsweringMachine, #$Telephone, #$LaserDiscPlayer, etc.</rdfs:comment>
        <rdfs:subClassOf rdf:resource="#ElectricalHouseholdAppliance"/>
        <rdfs:subClassOf rdf:resource="#ElectronicDevice"/>
    </owl:Class>

    <!-- All subClassOf associations checked -->
    <owl:Class rdf:ID="EncoderProgram">
        <rdfs:comment>The collection of all #$ComputerProgram-CWs whose
            purpose         is to perform an #$IBTRecoding with an
            #$InformationBearingThing         as its #$informationOrigin
            and a #$ComputerFileCopy containing the         same
            information as its #$fileCopyCreated. See #$DecoderProgram
            for programs going the other direction.</rdfs:comment>
        <rdfs:subClassOf rdf:resource="#UtilityProgram"/>
    </owl:Class>

    <!-- All subClassOf associations checked -->
    <owl:Class rdf:ID="Encoding">
        <rdfs:comment>The collection of events where some data in an
            #$InformationBearingThing are tranformed from a more
            &apos;raw&apos; or natural format to a more
            compressed/complex format.</rdfs:comment>
    </owl:Class>

    <!-- All subClassOf associations checked -->
    <owl:Class rdf:ID="Equalizer-AudioComponent">
        <rdfs:comment></rdfs:comment>
        <rdf:type rdf:resource="#ManufacturedGoodsType"/>
        <rdfs:subClassOf rdf:resource="#ManufacturedGoods"/>
        <rdfs:subClassOf rdf:resource="#AudioSystemComponent"/>
    </owl:Class>

    <!-- All subClassOf associations checked -->
    <owl:Class rdf:ID="Event">
        <rdfs:comment>An important specialization of #$Situation and
            thus also of #$IntangibleIndividual and
            #$TemporallyExistingThing (qq.v).  Each instance of #$Event
            is a dynamic situation in which the state of the world
            changes; each instance is something one would say  happens .
            Events are intangible because they are changes per se, not
            tangible objects that effect and undergo changes.    Notable
            specializations of #$Event include #$Event-Localized,
            #$PhysicalEvent, #$Action, and #$GeneralizedTransfer.
            #$Events should not be confused with #$TimeIntervals (q.v.).
            The temporal bounds of events are delineated by time
            intervals, but in contrast to many events time intervals
            have no spatial location or extent.</rdfs:comment>
    </owl:Class>

    <!-- All subClassOf associations checked -->
    <owl:Class rdf:ID="FlatPanelDisplay">
        <rdfs:comment>A specialization of #$ComputerMonitor-VideoKind.
            This is the collection of computer monitors that are a few
            inches deep, rather than the usual depth of more than a foot.</rdfs:comment>
        <rdf:type rdf:resource="#ManufacturedGoodsType"/>
        <rdfs:subClassOf rdf:resource="#ComputerMonitor-VideoKind"/>
        <rdfs:subClassOf rdf:resource="#ElectronicDisplayDevice"/>
    </owl:Class>

    <!-- All subClassOf associations checked -->
    <owl:Class rdf:ID="GeneralizedTransfer">
        <rdfs:comment>A specialization of #$Event.  Each instance of
            #$GeneralizedTransfer is an event in which something
            (tangible or intangible) is transferred from one
            `place&apos; to another.  #$GeneralizedTransfer includes
            changes in physical location, in ownership or possession,
            transfer of information, and propagation of wave phenomena
            through space.  See also the related predicate
            #$transferredThing, and the specializations of this collection.</rdfs:comment>
        <rdf:type rdf:resource="#DurativeEventType"/>
        <rdfs:subClassOf rdf:resource="#Event"/>
    </owl:Class>

    <!-- All subClassOf associations checked -->
    <owl:Class rdf:ID="Headphones">
        <rdfs:comment>The audio devices put very close to the ears to
            permit personal listening</rdfs:comment>
        <rdf:type rdf:resource="#ManufacturedGoodsType"/>
        <rdfs:subClassOf rdf:resource="#ManufacturedGoods"/>
        <rdfs:subClassOf rdf:resource="#ElectricalComponent"/>
    </owl:Class>

    <!-- All subClassOf associations checked -->
    <owl:Class rdf:ID="HomeAudioEquipment">
        <rdfs:comment>The subcollection of #$AudioEquipment instances of
            which are designed to be used in the home.</rdfs:comment>
        <rdfs:subClassOf rdf:resource="#AudioEquipment"/>
    </owl:Class>

    <!-- All subClassOf associations checked -->
    <owl:Class rdf:ID="HomeAudioReceiver">
        <rdfs:comment>A subcollection of both  #$Receiver-AudioComponent
            and #$HomeAudioSystemComponent. Instances of
            #$HomeAudioReceiver are meant to be components of instances
            of #$HomeAudioSystem.</rdfs:comment>
        <rdfs:subClassOf rdf:resource="#Receiver-AudioComponent"/>
        <rdfs:subClassOf rdf:resource="#HomeAudioSystemComponent"/>
    </owl:Class>

    <!-- All subClassOf associations checked -->
    <owl:Class rdf:ID="HomeAudioSystem">
        <rdfs:comment>The collection of #$AudioSystems designed and
            marketed for use in a home or office setting. Elements are
            usually assembled and left in a stationary position. Unlike
            elements of #$PortableAudioEquipment, they cannot be easily
            transported nor operated while in motion, although their
            positions in a room can be changed. Each instance of
            #$HomeAudioSystem has several instances of
            #$HomeAudioSystemComponent as #$physicalParts. No instance
            of #$HomeAudioSystemComponent is itself an instance of #$HomeAudioSystem.</rdfs:comment>
        <rdfs:subClassOf rdf:resource="#AudioSystem"/>
        <rdfs:subClassOf rdf:resource="#HomeAudioEquipment"/>
    </owl:Class>

    <!-- All subClassOf associations checked -->
    <owl:Class rdf:ID="HomeAudioSystemComponent">
        <rdfs:comment>The collection of #$AudioSystemComponents designed
            and marketed for use in a home or office setting. Elements
            of #$HomeAudioSystemComponent are typically purchased
            separately and assembled to form a #$HomeAudioSystem. Once
            assembled, the system is left in a stationary position for
            long periods of time. Unlike elements of
            #$PortableAudioEquipment, elements of
            #$HomeAudioSystemComponent cannot be easily transported nor
            operated while in motion, although their positions in a room
            can be changed. Thus, with respect to their relatively fixed
            positions once configured into a #$HomeAudioSystem, elements
            of #$HomeAudioSystemComponent are more like furniture than
            hand-held devices.</rdfs:comment>
        <rdfs:subClassOf rdf:resource="#AudioSystemComponent"/>
        <rdfs:subClassOf rdf:resource="#HomeAudioEquipment"/>
    </owl:Class>

    <owl:Class rdf:ID="HomeCDPlayer">
        <rdfs:comment>A subcollection of both #$CDPlayer-AudioComponent
            and #$HomeAudioSystemComponent. Instances of #$HomeCDPlayer
            are designed to be used in the home to play instances of #$CompactDisc-Generic.</rdfs:comment>
        <rdf:type rdf:resource="#ManufacturedGoodsType"/>
        <rdfs:subClassOf rdf:resource="#CDPlayer-AudioComponent"/>
        <rdfs:subClassOf rdf:resource="#HomeAudioSystemComponent"/>
    </owl:Class>

    <!-- All subClassOf associations checked -->    
    <owl:Class rdf:ID="HomeStereoSpeaker">
        <rdfs:comment>A subcollection of both #$HomeAudioSystemComponent
            and #$StereoSpeaker. Instances of #$HomeStereoSpeaker are
            designed to output sound as components of instances of  #$HomeAudioSystem.</rdfs:comment>
        <rdf:type rdf:resource="#ManufacturedGoodsType"/>
        <rdfs:subClassOf rdf:resource="#StereoSpeaker"/>
        <rdfs:subClassOf rdf:resource="#HomeAudioSystemComponent"/>
    </owl:Class>
    
    <!-- All subClassOf associations checked -->
    <owl:Class rdf:ID="HomeTheaterSystem">
        <rdfs:comment>This is the collection of home theater  systems.
            These are basically large-screen television sets souped-up
            with  some sort of hi-fi sound system.</rdfs:comment>
        <rdfs:subClassOf rdf:resource="#MechanicalDevice"/>
        <rdfs:subClassOf rdf:resource="#ElectricalDevice"/>
    </owl:Class>

    <!-- All subClassOf associations checked -->
    <owl:Class rdf:ID="HomeVideoGameMachine">
        <rdfs:comment>This is the device on which we affectionately play
            video games like Space Invaders or Asteroids.  This machine
            is hooked up to a televison set</rdfs:comment>
        <rdf:type rdf:resource="#ManufacturedGoodsType"/>
        <rdfs:subClassOf rdf:resource="#ManufacturedGoods"/>
        <rdfs:subClassOf rdf:resource="#ElectronicHouseholdAppliance"/>
    </owl:Class>

    <!-- All subClassOf associations checked -->
    <owl:Class rdf:ID="InformationStorageMedia">
        <rdfs:comment>Items which can have (but don&apos;t necessarily
            have) information stored onto them that can be retrieved later.</rdfs:comment>
    </owl:Class>

    <!-- All subClassOf associations checked -->
    <owl:Class rdf:ID="InformationTransferEvent">
        <rdfs:comment>A specialization of #$GeneralizedTransfer.  Each
            instance of #$InformationTransferEvent is an event in which
            information is transferred from a source
            (#$informationOrigin) to one or more destinations
            (#$informationDestination), where the source and the various
            destinations are either intelligent agents or
            #$InformationBearingThings (IBTs).  Examples include reading
            a book (transfer of information from the book to the
            reader), saying something to someone (transfer of
            information from the speaker to the listener), machine
            translation (transfer of information from an encoded IBT in
            the source language to an encoded IBT in the target
            language), OCR scanning (transfer of information from a
            visual information source to another IBT in a different
            format), carving initials in a tree (transfer of information
            from an agent to an IBT),  and making a speech (transfer of
            information from an agent to other agents).  See also the
            specialization #$InformationTransferPhysicalEvent.</rdfs:comment>
        <rdfs:subClassOf rdf:resource="#GeneralizedTransfer"/>
    </owl:Class>

    <!-- All subClassOf associations checked -->
    <owl:Class rdf:ID="InformationTransferEvent-Electronic">
        <rdfs:comment>The collection of all events in which information
            is transferred electronically. Examples include all
            instances of #$TelephoneConversation, #$EMailSending, and #$PuttingUpAWebsite.</rdfs:comment>
        <rdfs:subClassOf rdf:resource="#InformationTransferPhysicalEvent"/>
    </owl:Class>

    <!-- All subClassOf associations checked -->
    <owl:Class rdf:ID="InformationTransferPhysicalEvent">
        <rdfs:comment>A specialization of #$InformationTransferEvent
            (q.v.) and #$PhysicalEvent each instance of which involves
            at least one #$PartiallyTangible, either as its source (see
            #$informationOrigin), as (at least one of) its
            destination(s) (see #$informationDestination), or both.  (A
            partially tangible source or destination, note, must
            pre-exist the transfer event.)  Indeed, most if not all
            actual information transfer events are physical events; but
            #$InformationTransferPhysicalEvent does in principle exclude
            those such as telepathic communications between disembodied
            spirits or other #$Agent-Intangibles.</rdfs:comment>
        <rdfs:subClassOf rdf:resource="#PhysicalEvent"/>
        <rdfs:subClassOf rdf:resource="#InformationTransferEvent"/>
    </owl:Class>

    <!-- All subClassOf associations checked -->
    <owl:Class rdf:ID="InputDataStream">
        <rdfs:comment>This generic data type encapsluates the concept of
            input streams in programming languages.</rdfs:comment>
        <rdf:type rdf:resource="#ComputerDataType"/>
        <rdfs:subClassOf rdf:resource="#DataStream"/>
    </owl:Class>

    <!-- All subClassOf associations checked -->
    <owl:Class rdf:ID="Jukebox">
        <rdfs:comment>The collection of all jukeboxes. A #$Jukebox is a
            coin-operated CD- or record-playing machine, usually found
            in restaurants or bars.</rdfs:comment>
        <rdf:type rdf:resource="#ManufacturedGoodsType"/>
        <rdfs:subClassOf rdf:resource="#ManufacturedGoods"/>
        <rdfs:subClassOf rdf:resource="#AudioEquipment"/>
        <rdfs:subClassOf rdf:resource="#MediaPlayingDevice"/>
    </owl:Class>

    <!-- All subClassOf associations checked -->
    <owl:Class rdf:ID="LaserDiscPlayer">
        <rdfs:comment></rdfs:comment>
        <rdf:type rdf:resource="#ManufacturedGoodsType"/>
        <rdfs:subClassOf rdf:resource="#ManufacturedGoods"/>
        <rdfs:subClassOf rdf:resource="#ConsumerAudioVideoComponent"/>
        <rdfs:subClassOf rdf:resource="#MediaPlayingDevice"/>
    </owl:Class>

    <!-- All subClassOf associations checked -->
    <owl:Class rdf:ID="ManufacturedGoods">
        <rdfs:comment>The collection of all #$Artifacts that are made or
            processed in large-scale industrial operations for
            distribution (normally sale) to agents outside the
            manufacturing organization.  This includes manufactured
            stuff, e.g. Finlandia vodka; refined ore, e.g. iron;
            otherwise procesed natural material, e.g. cut diamonds, as
            well as manufactured objects.  This collection excludes
            handicrafts; privately made stuff, e.g. moonshine; and other
            artifacts produced by one or a few people on a small scale.</rdfs:comment>
    </owl:Class>

    <!-- All subClassOf associations checked -->
    <owl:Class rdf:ID="MechanicalDevice">
        <rdfs:comment>A specialization of #$PhysicalDevice.  Each
            instance of #$MechanicalDevice is a physical device which
            has at least one part that moves with respect to another one
            of its parts.  Thus a spoon is not an instance of
            #$MechanicalDevice, but a pair of scissors is, as are more
            complex devices such as vacuum cleaners and the #$SpaceShuttleChallenger.</rdfs:comment>
        <rdfs:subClassOf rdf:resource="#PhysicalDevice"/>
    </owl:Class>

    <!-- All subClassOf associations checked -->
    <owl:Class rdf:ID="MediaPlayingDevice">
        <rdfs:comment></rdfs:comment>
        <rdfs:subClassOf rdf:resource="#ElectronicDevice"/>
        <rdfs:subClassOf rdf:resource="#MechanicalDevice"/>
    </owl:Class>

    <!-- All subClassOf associations checked -->
    <owl:Class rdf:ID="MiniAudioSystem">
        <rdfs:comment></rdfs:comment>
        <rdfs:subClassOf rdf:resource="#AudioSystem"/>
    </owl:Class>

    <!-- All subClassOf associations checked -->
    <owl:Class rdf:ID="Mixer-AudioComponent">
        <rdfs:comment>A collection of audio equipment. Each instance of
            Mixer-AudioComponent accepts two or more inputs from audio
            devices,   microphones, etc. and has one or more output
            signal combining multiple   inputs.</rdfs:comment>
        <rdf:type rdf:resource="#ManufacturedGoodsType"/>
        <rdfs:subClassOf rdf:resource="#ManufacturedGoods"/>
        <rdfs:subClassOf rdf:resource="#AudioSystemComponent"/>
    </owl:Class>

    <!-- All subClassOf associations checked -->
    <owl:Class rdf:ID="MP3Player">
        <rdfs:comment>The collection of hardware devices whose primary
            intended purpose is to play MP3 files.  A computer is not an
            #$MP3Player (even if that&apos;s all it&apos;s used for)
            because that was not its primary intended purpose.</rdfs:comment>
        <rdf:type rdf:resource="#ManufacturedGoodsType"/>
        <rdfs:subClassOf rdf:resource="#ManufacturedGoods"/>
        <rdfs:subClassOf rdf:resource="#AudioEquipment"/>
        <rdfs:subClassOf rdf:resource="#MediaPlayingDevice"/>
        <rdfs:subClassOf rdf:resource="#MP3Player-Generic"/>
    </owl:Class>

    <!-- All subClassOf associations checked -->
    <owl:Class rdf:ID="MP3Player-Generic">
        <rdfs:comment>The collection of all things --- hardware or
            software --- whose primary intended purpose is to play MP3 files.</rdfs:comment>
        <rdfs:subClassOf rdf:resource="#TemporalThing"/>
    </owl:Class>

    <!-- All subClassOf associations checked -->
    <owl:Class rdf:ID="MusicVideoCopy">
        <rdfs:comment>A #$VideoRecordedObject whose playings (see
            #$performanceOfIBT) have an audio portion, consisting of a
            #$Song-Sung, and a video portion typically consisting of
            images of the performers dancing, singing, playing
            instruments, etc. Made for sale or television broadcast.</rdfs:comment>
        <rdfs:subClassOf rdf:resource="#VideoRecordedObject"/>
    </owl:Class>

    <!-- All subClassOf associations checked -->
    <owl:Class rdf:ID="OutputDataStream">
        <rdfs:comment>This generic data type encapsluates the concept of
            output streams in programming languages.</rdfs:comment>
        <rdf:type rdf:resource="#ComputerDataType"/>
        <rdfs:subClassOf rdf:resource="#DataStream"/>
    </owl:Class>

    <!-- All subClassOf associations checked -->
    <owl:Class rdf:ID="PackagedAudioHomeTheater">
        <rdfs:comment>A subcollection of #$HomeAudioSystem. Instances of
            #$PackagedAudioHomeTheatre are on the expensive and
            physically large end. They typically have surround sound
            speakers and a logic processor for DVD</rdfs:comment>
        <rdf:type rdf:resource="#ManufacturedGoodsType"/>
        <rdfs:subClassOf rdf:resource="#ManufacturedGoods"/>
        <rdfs:subClassOf rdf:resource="#HomeAudioSystem"/>
    </owl:Class>

    <!-- All subClassOf associations checked -->
    <owl:Class rdf:ID="PersonalAudioPlayer">
        <rdfs:comment>#$PersonalAudioPlayer is a collection of
            #$PortableAudioEquipment that is designed for use by a
            single person using #$Headphones. Elements of
            #$PortableAudioEquipment are designed to be both compact in
            size and light in weight. As a result, they can be used in
            activities in which they are strapped to the user&apos;s
            body, e.g., during jogging and exercise workouts.</rdfs:comment>
        <rdf:type rdf:resource="#ManufacturedGoodsType"/>
        <rdfs:subClassOf rdf:resource="#Device-SingleUser"/>
        <rdfs:subClassOf rdf:resource="#PortableAudioEquipment"/>
    </owl:Class>

    <!-- All subClassOf associations checked -->
    <owl:Class rdf:ID="PersonalDevice">
        <rdfs:comment>The collection of devices that are controlled and
            primarily used by one person, and which are often carried by
            the person rather than permanently situated in a particular
            #$HumanOccupationConstruct. Not included are household
            devices, which are often shared by more than one dweller in
            a #$HumanResidence. Also not included are instances of
            #$BusinessMachine, as these are often shared by multiple
            coworkers. Specializations include #$Pager, #$Wallet and
            #$CellularTelephone. #$PersonalDevice differs from
            #$Device-SingleUser in that an instance of the latter can
            typically be shared among more than one user, as long as it
            is not used by both users simultaneously. Neither
            #$PersonalComputer nor #$LaptopComputer are specializations
            of #$PersonalDevice (both are often shared by multiple
            people, though not simultaneously), but certain instances of
            LaptopComputer might also be instances of #$PersonalDevice.</rdfs:comment>
        <rdfs:subClassOf rdf:resource="#PortableObject"/>
    </owl:Class>

    <!-- All subClassOf associations checked -->
    <owl:Class rdf:ID="PersonalDigitalAudioPlayer">
        <rdfs:comment>A subcollection of #$PersonalAudioPlayer.
            Instances of #$PersonalDigitalAudioPlayer are designed to
            convert instances of #$ComputerSoundFile (not stored on
            instances of #$CompactDisc-Generic) into instances of #$AudibleSound.</rdfs:comment>
        <rdf:type rdf:resource="#ManufacturedGoodsType"/>
        <rdfs:subClassOf rdf:resource="#PersonalAudioPlayer"/>
        <rdfs:subClassOf rdf:resource="#PersonalDevice"/>
    </owl:Class>

    <owl:Class rdf:ID="PersonalMP3Player">
        <rdfs:comment>A subcollection of #$PersonalDigitalAudioPlayer.
            Instances of #$PersonalMP3Player are designed to convert
            instances of #$MP3File (not stored on instances of
            #$CompactDisc-Generic) into instances of #$AudibleSound.</rdfs:comment>
        <rdf:type rdf:resource="#ManufacturedGoodsType"/>
        <rdfs:subClassOf rdf:resource="#PersonalDigitalAudioPlayer"/>
        <rdfs:subClassOf rdf:resource="#MP3Player"/>
    </owl:Class>

    <owl:Class rdf:ID="PersonalRadio">
        <rdfs:comment>A subcollection of both #$Radio and
            #$PersonalAudioPlayer. Instances of #$PersonalRadio convert
            instances of #$RadioWave into instances of #$AudibleSound,
            and are small and portable enough to use while jogging.</rdfs:comment>
        <rdf:type rdf:resource="#ManufacturedGoodsType"/>
        <rdfs:subClassOf rdf:resource="#Radio"/>
        <rdfs:subClassOf rdf:resource="#PersonalAudioPlayer"/>
    </owl:Class>

    <!-- All subClassOf associations checked -->
    <owl:Class rdf:ID="PhysicalDevice">
        <rdfs:comment>A specialization of #$Artifact and
            #$ObjectWithUse. Each instance of #$PhysicalDevice is an
            artifact with a relatively rigid, set shape, designed for a
            specific use or to perform a specific function.
            Specializations of #$PhysicalDevice thus include (among
            others) #$RoadVehicle, #$Motorboat, #$HandTool, and
            #$PlumbingFixture.  Note that artifacts which are only to be
            viewed or can only be  used  in a very loose or metaphorical
            sense, such as instances of #$Buoy, #$Sculpture,
            #$FlowerBed, or #$Billboard, are _not_ instances of
            #$PhysicalDevice.  Moreover, artifacts which have a specific
            use or function, but which do not have a relatively rigid,
            set shape are _not_ instances of #$PhysicalDevice; for this
            reason, neither #$GasolineFuel nor #$AntiFreeze are
            specializations of #$PhysicalDevice.</rdfs:comment>
        <rdfs:subClassOf rdf:resource="#SinglePurposeDevice"/>
    </owl:Class>

    <!-- All subClassOf associations checked -->
    <owl:Class rdf:ID="PhysicalEvent">
        <rdfs:comment>A specialization of #$Event-Localized.  Each
            instance of #$PhysicalEvent is a spatially localized event
            involving one or more physical objects or stuffs.
            #$PhysicalEvents typically involve interaction among
            #$PartiallyTangibles.  But note that a physical event might
            consist in the creation, destruction, movement, or a change
            in some physical feature of a single salient physical
            object.  (See #$PhysicalCreationEvent,
            #$PhysicalDestructionEvent, #$MovementEvent, and
            #$IntrinsicStateChangeEvent.)  For a contrasting (though not
            necessarily disjoint) collection, see #$StrictlyMentalEvent.
            For events that have both physical and mental components,
            see the collection #$CompositePhysicalAndMentalEvent.</rdfs:comment>
    </owl:Class>

    <!-- All subClassOf associations checked -->
    <owl:Class rdf:ID="PortableAudioEquipment">
        <rdfs:comment>The collection of #$AudioSystems which are also
            #$PortableObjects and#$SelfPoweredDevices. What makes an
            instance of #$AudioSystem portable or mobile is that it is
            both lightweight enough to be carried easily by a #$Person
            and  can be operated without requiring that it be plugged
            into a external power source. A device can be an instance of
            #$PortableAudioEquipment even if it can be operated by an
            external power source, as long as it is also an instance of
            #$SelfPoweredDevice. A positive example is a #$Walkman. A
            negative example is a #$CompactDiscPlayer that is part of a
            home entertainmnet audio system (#$HomeAudioSystem).</rdfs:comment>
        <rdf:type rdf:resource="#ManufacturedGoodsType"/>
        <rdfs:subClassOf rdf:resource="#ManufacturedGoods"/>
        <rdfs:subClassOf rdf:resource="#AudioSystem"/>
        <rdfs:subClassOf rdf:resource="#PortableObject"/>
    </owl:Class>

    <owl:Class rdf:ID="PortableCDPlayer">
        <rdfs:comment></rdfs:comment>
        <rdf:type rdf:resource="#ManufacturedGoodsType"/>
        <rdfs:subClassOf rdf:resource="#CompactDiscPlayer"/>
        <rdfs:subClassOf rdf:resource="#PersonalAudioPlayer"/>
    </owl:Class>

    <owl:Class rdf:ID="PortableObject">
        <rdfs:comment>A specialization of #$HumanScaleObject.  Each
            instance of #$PortableObject is a tangible object that is
            not  fastened down  and is light enough for an average human
            (or, more to the point, for its average intended user) to
            move easily.  For many instances of #$PortableObject,
            portability is important for the fulfillment of their
            primary functions;  for example, an article of clothing (an
            instance of #$SomethingToWear),  a hand-guided tool (an
            instance of #$HandTool), a coin or dollar bill (an instance
            of #$Currency), or a flashlight (an instance of
            #$Flashlight) would be pretty useless if they weren&apos;t
            portable.  In other cases, making a device portable, or
            making a portable version of a device, simply provides a
            convenience, as with the subcollections #$PortableTelevision
            and #$PortableStereoSystem.  Note that #$Tool is not a
            subcollection of #$PortableObject, since many tools are
            heavy and/or stationary.  A borderline example of a
            #$PortableObject would be a heart/lung machine; although the
            beneficiary of its primary function is in no position to
            move it around, the physicians and nurses who also are
            using  it can and do exactly that.  The same goes for a
            playpen; the kids in it had better _not_ be able to move it
            around, but the adults who set it up and put them there can
            and do move it.   A borderline non-example would be a car;
            even though its user can make it move around, that is more a
            controlling action than a transporting action --- i.e., the
            car is doing the transporting in that case, not the driver.
            A borderline example is a cat; even though it moves under
            its own power, it is light enough for its owner to pick it
            up and move it around.  A borderline example is a bed or a
            dresser; though too heavy to lift, its owners can generally
            move it around (by sliding, disassembling and reassembling,
            and so on).</rdfs:comment>
    </owl:Class>

    <!-- All subClassOf associations checked -->
    <owl:Class rdf:ID="PoweredDevice">
        <rdfs:comment>A specialization of #$PhysicalDevice.  Each
            instance of #$PoweredDevice is a device that requires some
            power input in order to perform its intended function(s).
            The power supplied might be muscle power, kinetic energy,
            electricity, fuel-generated, and so on.  Note that
            #$PoweredDevice and #$NonPoweredDevice partition the
            collection #$PhysicalDevice.</rdfs:comment>
        <rdfs:subClassOf rdf:resource="#PhysicalDevice"/>
    </owl:Class>

    <!-- All subClassOf associations checked -->
    <owl:Class rdf:ID="ProgramObject">
        <rdfs:comment>A specialization of #$ComputerAIS. #$ProgramObject
            is the collection of all data structures that are explicitly
            referenced in computer programs. All data types are
            considered to be specializations of this collection.</rdfs:comment>
        <rdf:type rdf:resource="#ComputerDataType"/>
    </owl:Class>

    <!-- All subClassOf associations checked -->
    <owl:Class rdf:ID="ProjectionDisplayDevice">
        <rdfs:comment>Devices which display images via projection onto a screen.</rdfs:comment>
        <rdf:type rdf:resource="#ManufacturedGoodsType"/>
        <rdfs:subClassOf rdf:resource="#ElectronicDisplayDevice"/>
    </owl:Class>

    <!-- All subClassOf associations checked -->
    <owl:Class rdf:ID="ProjectionTelevision">
        <rdfs:comment></rdfs:comment>
        <rdf:type rdf:resource="#ManufacturedGoodsType"/>
        <rdfs:subClassOf rdf:resource="#TelevisionSet"/>
    </owl:Class>

    <!-- All subClassOf associations checked -->
    <owl:Class rdf:ID="Radio">
        <rdfs:comment>A subcollection of #$WirelessCommunicationDevice.
            Instances of #$Radio convert instances of #$RadioWave into
            instances of #$AudibleSound.</rdfs:comment>
        <rdfs:subClassOf rdf:resource="#AudioSystem"/>
        <rdfs:subClassOf rdf:resource="#WirelessCommunicationDevice"/>
    </owl:Class>

    <!-- All subClassOf associations checked -->
    <owl:Class rdf:ID="RadioReceiver">
        <rdfs:comment>The device used to receive transmissions broadcast
            in radio frequencies (does not include radio transmitters).</rdfs:comment>
        <rdfs:subClassOf rdf:resource="#WirelessCommunicationDevice"/>
    </owl:Class>

    <!-- All subClassOf associations checked -->
    <owl:Class rdf:ID="Receiver-AudioComponent">
        <rdfs:comment>The receiver component of a component stereo
            system. Other #$AudioSystemComponents outputs feed into the
            #$Receiver-AudioComponent which in turn drives the #$AudioSpeakers.</rdfs:comment>
        <rdfs:subClassOf rdf:resource="#RadioReceiver"/>
        <rdfs:subClassOf rdf:resource="#ConsumerAudioVideoComponent"/>
        <rdfs:subClassOf rdf:resource="#AudioSystemComponent"/>
    </owl:Class>

    <!-- All subClassOf associations checked -->
    <owl:Class rdf:ID="SatelliteTVReceiver">
        <rdfs:comment>The collection of all satellite television
            receivers. Instances are generally black boxes with remote
            controls that take as input a signal from a
            #$SatelliteTVAntenna, tune in a channel, and pass video and
            audio signals out to a #$TelevisionSet,
            #$Receiver-AudioComponent, etc.</rdfs:comment>
        <rdf:type rdf:resource="#ManufacturedGoodsType"/>
        <rdfs:subClassOf rdf:resource="#ManufacturedGoods"/>
        <rdfs:subClassOf rdf:resource="#ConsumerAudioVideoComponent"/>
    </owl:Class>

    <!-- All subClassOf associations checked -->
    <owl:Class rdf:ID="SinglePurposeDevice">
        <rdfs:comment>A collection of devices each of which has a single
            #$primaryFunction.   Each instance of #$SinglePurposeDevice
            may have more than one function, but will have only one
            _primary_ function.  For example, a car is a single purpose
            device because it has the primary function of providing
            transportation.  Of course, a car can provide shelter as
            well as transportation; but a convertible with a badly torn
            roof still functions as a car (because its primary function
            is transportation) even though it does not function as much
            of a shelter.  It is also possible for a
            #$SinglePurposeDevice to have other functions associated
            with it, even though they are not functions of that device
            per se.  For example, if a car has a cigarette lighter, a
            clock, etc., those parts have their own functions, which are
            performed in the car and enjoyed by the users of the car
            while they are using the car.  However, the functions of
            those devices (lighting cigarettes and telling time) are
            generally not considered to be the functions of the car
            itself.  If someone utters the sentence `Fred used his car
            today&apos; we would guess that Fred drove/rode somewhere in
            the car, and would be surprised/amused/annoyed/confused if
            we later discover that the speaker meant only that Fred used
            the car&apos;s lighter and the clock but didn&apos;t travel
            somewhere by car.</rdfs:comment>
        <rdfs:subClassOf rdf:resource="#PhysicalDevice"/>
    </owl:Class>

    <!-- All subClassOf associations checked -->
    <owl:Class rdf:ID="Stereophonic">
        <rdfs:comment>An attribute of audio or audio-visual components
            or systems. Any stereo component or system is capable of
            processing 2-channel sound signals intended for left and
            right speakers.</rdfs:comment>
        <rdfs:subClassOf rdf:resource="#ElectronicDevice"/>
    </owl:Class>

    <!-- All subClassOf associations checked -->
    <owl:Class rdf:ID="StereoSpeaker">
        <rdfs:comment>The speaker which produces the sound from a stereo
            system.  It usually includes some sort of cubical housing</rdfs:comment>
        <rdf:type rdf:resource="#ManufacturedGoodsType"/>
        <rdfs:subClassOf rdf:resource="#AudioSystemComponent"/>
        <rdfs:subClassOf rdf:resource="#AudioSpeaker"/>
    </owl:Class>

    <!-- All subClassOf associations checked -->
    <owl:Class rdf:ID="StereoSystem">
        <rdfs:comment>A collection of audio systems. Each instance of
            StereoSystem is capable of reproducting 2-channel sound.</rdfs:comment>
        <rdfs:subClassOf rdf:resource="#AudioSystem"/>
        <rdfs:subClassOf rdf:resource="#Stereophonic"/>
    </owl:Class>

    <!-- All subClassOf associations checked -->
    <owl:Class rdf:ID="Subwoofer">
        <rdfs:comment>A specialized #$StereoSpeaker responsible for
            producing deep bass.</rdfs:comment>
        <rdf:type rdf:resource="#ManufacturedGoodsType"/>
        <rdfs:subClassOf rdf:resource="#AudioSystemComponent"/>
        <rdfs:subClassOf rdf:resource="#AudioSpeaker"/>
    </owl:Class>

    <!-- All subClassOf associations checked -->
    <owl:Class rdf:ID="System">
        <rdfs:comment>The collection of all systems -- complex objects
            that decompose into simpler components that, by virtue of
            the relations among them, form a recognizable, cohesive
            whole.  Notable specializations include #$PathSystem and
            #$FunctionalSystem.  The components of an instance of
            #$System can be identified using #$systemComponents.</rdfs:comment>
        <rdfs:subClassOf rdf:resource="http://www.w3.org/2002/07/owl#Thing"/>
    </owl:Class>

    <!-- All subClassOf associations checked -->
    <owl:Class rdf:ID="TelevisionSet">
        <rdfs:comment>A television set</rdfs:comment>
        <rdf:type rdf:resource="#ManufacturedGoodsType"/>
        <rdfs:subClassOf rdf:resource="#ManufacturedGoods"/>
        <rdfs:subClassOf rdf:resource="#ElectronicHouseholdAppliance"/>
        <rdfs:subClassOf rdf:resource="#CommunicationDevice"/>
    </owl:Class>

    <!-- All subClassOf associations checked -->
    <owl:Class rdf:ID="TelevisionTuner">
        <rdfs:comment>Television tuners do for television signals what
            radio tuners do for radio broadcasts.</rdfs:comment>
        <rdf:type rdf:resource="#ManufacturedGoodsType"/>
        <rdfs:subClassOf rdf:resource="#VideoReceiverComponent"/>
    </owl:Class>

    <!-- All subClassOf associations checked -->
    <owl:Class rdf:ID="Transmitter">
        <rdfs:comment>Device used for transmitting radio or tv signals.</rdfs:comment>
        <rdfs:subClassOf rdf:resource="#WirelessCommunicationDevice"/>
        <rdfs:subClassOf rdf:resource="#ElectronicComponent"/>
    </owl:Class>

    <!-- All subClassOf associations checked -->
    <owl:Class rdf:ID="UtilityProgram">
        <rdfs:comment>Software which allows a user to manage a variety
            of aspects of their computer, such as decompressing files,
            memory management, hard drive scanning, anti-viral programs,
            etc. See also #$AdministrationProgram, #$BackEndUtilityProgram.</rdfs:comment>
        <rdf:type rdf:resource="#ComputerProgramTypeByFunction"/>
    </owl:Class>

    <owl:Class rdf:ID="VideoProjector">
        <rdfs:comment>Stand alone devices which take inputs from
            various electronic video sources (S-Video, computer video
            cards, etc.)   and not #$MovieReels.  Therefore, a negative
            example would of course be   #$MovieProjector.</rdfs:comment>
        <rdf:type rdf:resource="#ManufacturedGoodsType"/>
        <rdfs:subClassOf rdf:resource="#ProjectionDisplayDevice"/>
    </owl:Class>

    <!-- All subClassOf associations checked -->
    <owl:Class rdf:ID="VideoRecordedObject">
        <rdfs:comment>A collection of information bearing objects
            (IBOs).  Each element of #$VideoRecordedObject is a tangible
            object (such as a videotape) that contains visual
            information.  For mass-produced videos, see #$RecordedVideoProduct.</rdfs:comment>
    </owl:Class>

    <!-- All subClassOf associations checked -->
    <owl:Class rdf:ID="VideoReceiverComponent">
        <rdfs:comment>Electronic Device which receives video signals and
            decodes them into signals of visual images which can be
            amplified for display.  See also Television and #$VideoCassetteRecorder</rdfs:comment>
        <rdf:type rdf:resource="#ManufacturedGoodsType"/>
        <rdfs:subClassOf rdf:resource="#ManufacturedGoods"/>
        <rdfs:subClassOf rdf:resource="#ElectronicComponent"/>
    </owl:Class>

    <!-- All subClassOf associations checked -->
    <owl:Class rdf:ID="VideoScreen">
        <rdfs:comment>A video display screen for a piece of electronic hardware</rdfs:comment>
        <rdf:type rdf:resource="#ManufacturedGoodsType"/>
        <rdfs:subClassOf rdf:resource="#ManufacturedGoods"/>
        <rdfs:subClassOf rdf:resource="#ElectricalComponent"/>
    </owl:Class>

    <owl:Class rdf:ID="Walkman">
        <rdfs:comment></rdfs:comment>
        <rdf:type rdf:resource="#ProductTypeByBrand"/>
        <rdf:type rdf:resource="#ManufacturedGoodsType"/>
        <rdfs:subClassOf rdf:resource="#PersonalAudioPlayer"/>
        <rdfs:subClassOf rdf:resource="#PortableObject"/>
        <rdfs:subClassOf rdf:resource="#StereoSystem"/>
    </owl:Class>

    <owl:Class rdf:ID="Walkman-RadioOnly">
        <rdfs:comment></rdfs:comment>
        <rdf:type rdf:resource="#ProductTypeByBrand"/>
        <rdf:type rdf:resource="#ManufacturedGoodsType"/>
        <rdfs:subClassOf rdf:resource="#PersonalRadio"/>
        <rdfs:subClassOf rdf:resource="#Walkman"/>
        <rdfs:subClassOf rdf:resource="#RadioReceiver"/>
    </owl:Class>

    <!-- All subClassOf associations checked -->
    <owl:Class rdf:ID="WirelessCommunicationDevice">
        <rdfs:comment>The collection of   #$CommunicationDevices in
            which the communication signals are either not transmitted
            or not received entirely over a wire.</rdfs:comment>
        <rdfs:subClassOf rdf:resource="#CommunicationDevice"/>
        <rdfs:subClassOf rdf:resource="#ElectronicDevice"/>
    </owl:Class>

    <!--Object Properties -->
    <owl:ObjectProperty rdf:ID="decodingDeviceType">
        <rdfs:comment>This predicate is used to specify the type of
            device needed for decoding information contained in a
            particular kind of encoding scheme.  (#$decodingDeviceType
            SCHEME DEV-TYP) means that DEV-TYP is the type of device
            required to decode the information encoded with encoding
            scheme SCHEME.  For example, a telephone is the kind of
            device needed to decode audio information sent over
            telephone lines.  A cable TV box is the device type needed
            to decode cable TV signals.  And so on.  See also #$EncodingSchemeType.</rdfs:comment>
    </owl:ObjectProperty>

    <owl:ObjectProperty rdf:ID="infoTransferred">
        <rdfs:comment>A #$BinaryRolePredicate that is used to specify
            some or all of the meaningful content of a particular
            transferral of information (see
            #$InformationTransferEvent).  (#$infoTransferred TRANSFER
            INFO) means  that INFO is information (see
            #$AspatialInformationStore) that is  transferred due to
            TRANSFER.  INFO originates (see #$informationOrigin) from
            some agent or #$InformationBearingThing (IBT) and, after
            TRANSFER,  is had by another agent or is contained in
            another IBT (see  #$informationDestination); INFO may
            persist in the origin as well.  For example, when I read the
            front page of the newspaper, some  information about current
            world events is transferred from the  newspaper to me.</rdfs:comment>
        <rdfs:subPropertyOf rdf:resource="#situationConstituents"/>
    </owl:ObjectProperty>

    <owl:ObjectProperty rdf:ID="informationDestination">
        <rdfs:comment>A specialization of both #$informationTerminal and
            #$to-Generic that is used to  indicate where information is
            transferred in a given #$InformationTransferEvent.
            (#$informationDestination TRANSFER DESTINATION) means that
            in TRANSFER, the  information being transferred is sent to,
            given to, or impressed upon DESTINATION. DESTINATION is
            typically either an #$InformationBearingThing (at least upon
            the completion of TRANSFER, if not before) or an agent; but
            note that  in the latter case one would normally use the
            more specific predicate  #$recipientOfInfo.</rdfs:comment>
        <rdfs:subPropertyOf rdf:resource="#to-Generic"/>
        <rdfs:subPropertyOf rdf:resource="#informationTerminal"/>
    </owl:ObjectProperty>

    <owl:ObjectProperty rdf:ID="informationOrigin">
        <rdfs:comment>A specialization of #$informationTerminal  (q.v.)
            that is used to indicate the source of information for a
            particular  #$InformationTransferEvent (q.v.).
            (#$informationOrigin TRANSFER ORIGIN)  means that the
            information being transferred in TRANSFER comes from ORIGIN.
            ORIGIN is either an instance of #$InformationBearingThing or
            an agent.   Note that if ORIGIN still exists after the
            ending of TRANSFER, it  presumably also still contains the
            information that was transferred.</rdfs:comment>
        <rdfs:subPropertyOf rdf:resource="#from-Generic"/>
        <rdfs:subPropertyOf rdf:resource="#informationTerminal"/>
    </owl:ObjectProperty>

    <owl:ObjectProperty rdf:ID="informationTerminal">
        <rdfs:comment>This predicate is used to indicate any instance of
            #$TemporalThing the plays            the role of either
            #$informationDestination or #$informationOrigin in any
            instance of #$InformationTransferEvent, i.e. plays the role
            of endpoint.  (#$informationTerminal TRANS THING)
            means the #$TemporalThing THING was either the origin or
            destination            of the #$InformationTransferEvent TRANS.</rdfs:comment>
        <rdfs:subPropertyOf rdf:resource="#terminalOfTrans-Generic"/>
    </owl:ObjectProperty>
</rdf:RDF>